It might work
I found a way to prove well-foundedness for rose trees and it works,
but the same strategy fails for my patterns.

But I found that if I define a dependent rose tree, *similar* to
the application pattern, it does work. So I'm starting over in a clean
file, making it incrementally more complex to see *where* it fails.
Also the original file is way too crowded.

I'm also using the Arguments command liberally to hopefully make it
easier to deal with the dependent stuff. It's not harming me so far.

TODO: replace OpmlPattern.v with doover.v and delete RT.v when done

matching-logic/src/OPML/OpmlPattern.v
@@ -42,7 +42,7 @@ Inductive OPMLPattern {Σ : OPMLSignature} : opml_sort -> Type :=
   | op_mu {s : opml_sort} (φ : OPMLPattern s) : OPMLPattern s
 .
 
-Inductive Edbi2 {Σ : OPMLSignature} : list opml_sort -> opml_sort -> Set :=
+Inductive Edbi2 {Σ : OPMLSignature} : list opml_sort -> opml_sort -> Type :=
   | edbi0 {s : opml_sort} {ss : list opml_sort} : Edbi2 (s :: ss) s
   | edbis {s s' : opml_sort} {ss : list opml_sort} : Edbi2 ss s -> Edbi2 (s' :: ss) s
 .
@@ -130,6 +130,8 @@ Inductive OPMLClosedPattern {Σ : OPMLSignature} : opml_sort -> list opml_sort -
   | ocp_fsvar {s : opml_sort} {ex mu : list opml_sort} (X : opml_svar s) : OPMLClosedPattern s ex mu
   | ocp_imp {s : opml_sort} {ex mu : list opml_sort} (φ1 : OPMLClosedPattern s ex mu) (φ2 : OPMLClosedPattern s ex mu) : OPMLClosedPattern s ex mu
   | ocp_app {ex mu : list opml_sort} (σ : opml_symbol) (args : @dephlist _ (OPMLClosedPattern ^~ ex ^~ mu) (opml_arg_sorts σ)) : OPMLClosedPattern (opml_ret_sort σ) ex mu
+  (* | ocp_app {ex mu : list opml_sort} (σ : opml_symbol) : foldr (λ c a, OPMLClosedPattern c ex mu -> a) (OPMLClosedPattern (opml_ret_sort σ) ex mu) (opml_arg_sorts σ) *)
+  (* | ocp_app {ex mu : list opml_sort} (σ : opml_symbol) (args : foldr (λ c a, (OPMLClosedPattern c ex mu * a)%type) unit (opml_arg_sorts σ)) : OPMLClosedPattern (opml_ret_sort σ) ex mu *)
   | ocp_ex {s s' : opml_sort} {ex mu : list opml_sort} (φ : OPMLClosedPattern s (s' :: ex) mu) : OPMLClosedPattern s ex mu
   | ocp_mu {s s' : opml_sort} {ex mu : list opml_sort} (φ : OPMLClosedPattern s ex (s' :: mu)) : OPMLClosedPattern s ex mu
 .
@@ -268,7 +270,58 @@ Proof.
   repeat constructor.
 Qed.
 
+Fixpoint dephlistIn' {A : Type} {F : A -> Type} {x : A} {xs : list A} {ED : EqDecision A} (y : F x) (ys : @dephlist A F xs) : Prop :=
+  match ys with
+  | dhnil => False
+  | @dhcons _ _ x' _ y' ys => match decide (x = x') with
+                              | left e => eq_rect x F y _ e = y'
+                              | right _ => False
+                              end \/ dephlistIn' y ys
+  end.
+
+Arguments dephlistIn' {_} {_} {_} {_} {_} & _ _ /.
+
+Goal @dephlistIn' bool (bool_rect _ nat bool) true [true; false; true; true; false] _ 5 ([4; true; 3; 5; false] : @dephlist _ (bool_rect _ nat bool) [true; false; true; true; false]).
+Proof.
+  cbv. auto.
+Qed.
+
 Definition thing {Σ : OPMLSignature} : Type := sigT (λ '(s, ex, mu), OPMLClosedPattern s ex mu).
+
+(* Lemma OPMLClosedPattern_custom_ind : *)
+(*   ∀ (Σ : OPMLSignature) (P : ∀ (o : opml_sort) (l l0 : list opml_sort), *)
+(*   OPMLClosedPattern o l l0 → Prop), *)
+(*   (∀ (ex mu : list opml_sort) (from to : opml_sort) (subsort : opml_subsort from to) (φ : OPMLClosedPattern from ex mu), P from ex mu φ → P to ex mu (ocp_upcast from to subsort φ)) → *)
+(*   (∀ (s : opml_sort) (ex mu : list opml_sort), P s ex mu ocp_bot) → *)
+(*   (∀ (s : opml_sort) (ex mu : list opml_sort) (dbi : Edbi2 ex s), P s ex mu (ocp_bevar dbi)) → *)
+(*   (∀ (s : opml_sort) (ex mu : list opml_sort) (dbi : Edbi2 mu s), P s ex mu (ocp_bsvar dbi)) → *)
+(*   (∀ (s : opml_sort) (ex mu : list opml_sort) (x : opml_evar s), P s ex mu (ocp_fevar x)) → *)
+(*   (∀ (s : opml_sort) (ex mu : list opml_sort) (X : opml_svar s), P s ex mu (ocp_fsvar X)) → *)
+(*   (∀ (s : opml_sort) (ex mu : list opml_sort) (φ1 : OPMLClosedPattern s ex mu), P s ex mu φ1 → ∀ φ2 : OPMLClosedPattern s ex mu, P s ex mu φ2 → P s ex mu (ocp_imp φ1 φ2)) → *)
+(*   (∀ (ex mu : list opml_sort) (σ : opml_symbol) (args : dephlist (opml_arg_sorts σ)), (∀ s φ, @dephlistIn' _ _ s _ _ φ args -> P s ex mu φ) -> P (opml_ret_sort σ) ex mu (ocp_app σ args)) → *)
+(*   (∀ (s s' : opml_sort) (ex mu : list opml_sort) (φ : OPMLClosedPattern s (s' :: ex) mu), P s (s' :: ex) mu φ → P s ex mu (ocp_ex φ)) → *)
+(*   (∀ (s s' : opml_sort) (ex mu : list opml_sort) (φ : OPMLClosedPattern s ex (s' :: mu)), P s ex (s' :: mu) φ → P s ex mu (ocp_mu φ)) → *)
+(*   ∀ (o : opml_sort) (l l0 : list opml_sort) (o0 : OPMLClosedPattern o l l0), P o l l0 o0. *)
+(* Proof. *)
+(*   intros * Hupcast Hbot Hbevar Hbsvar Hfevar Hfsvar Himp Happ Hex Hmu *. *)
+(*   destruct o0. *)
+(*   (1* dependent induction o0. *1) *)
+(*   (1* apply Hupcast. exact IHo0. *1) *)
+(*   8: { *)
+(*     apply Happ. intros. *)
+(*     clear Hupcast Hbot Hbevar Hbsvar Hfevar Hfsvar Himp Happ Hex Hmu. *)
+(*     (1* generalize dependent args. *1) *)
+(*     (1* fix IHargs 1. destruct args; intros. *1) *)
+(*     induction args; intros. *)
+(*     simpl in H. destruct H. *)
+(*     simpl in H. destruct H. *)
+(*     2: apply IHargs, H. *)
+(*     case_match. 2: destruct H. *)
+
+(* Goal forall {Σ : OPMLSignature} (P : thing -> Prop), forall ex mu σ args, (forall s φ, @dephlistIn' _ _ s (opml_arg_sorts σ) _ φ args -> P (existT (s, ex, mu) φ)) -> P (existT (opml_ret_sort σ, ex, mu) (ocp_app σ args)). *)
+(* Proof. *)
+(*   intros. *)
+(*   dependent induction args. *)
 
 Inductive SubPatternOf {Σ : OPMLSignature} : thing -> thing -> Prop :=
   | sp_upcast from to subsort ex mu φ : SubPatternOf (existT (from, ex, mu) φ) (existT (to, ex, mu) (ocp_upcast from to subsort φ))
@@ -295,10 +348,90 @@ Proof.
   repeat constructor.
 Qed.
 
-Print Acc.
+Definition SubPatternOf' {Σ : OPMLSignature} : relation thing.
+Proof.
+  intros [[[s ex] mu] φ] [[[s' ex'] mu'] φ'].
+  destruct φ'.
+  2-6: exact False.
+  - refine (match (decide ((s, ex, mu) = (from, ex0, mu0))) with
+            | left e => eq_rect (s, ex, mu) (uncurry3 OPMLClosedPattern) φ _ e = φ'
+            | right _ => False
+            end).
+  - refine (match (decide ((s, ex, mu) = (s0, ex0, mu0))) with
+            | left e => eq_rect (s, ex, mu) (uncurry3 OPMLClosedPattern) φ _ e = φ'1 \/ eq_rect (s, ex, mu) (uncurry3 OPMLClosedPattern) φ _ e = φ'2
+            | right _ => False
+            end).
+  - refine (match (decide ((ex, mu) = (ex0, mu0))) with
+            | left e => let asd : OPMLClosedPattern s ex0 mu0 := (eq_rect (ex, mu) (uncurry (OPMLClosedPattern s)) φ _ e) in dephlistIn' asd args
+            | right _ => False
+            end).
+  - refine (match (decide ((s, ex, mu) = (s0, s' :: ex0, mu0))) with
+            | left e => eq_rect (s, ex, mu) (uncurry3 OPMLClosedPattern) φ _ e = φ'
+            | right _ => False
+            end).
+  - refine (match (decide ((s, ex, mu) = (s0, ex0, s' :: mu0))) with
+            | left e => eq_rect (s, ex, mu) (uncurry3 OPMLClosedPattern) φ _ e = φ'
+            | right _ => False
+            end).
+Defined.
+
+Arguments SubPatternOf' {_} _ _ /.
+
+Goal forall {Σ : OPMLSignature}, well_founded SubPatternOf'.
+Proof.
+  intro.
+  unfold well_founded.
+  fix pleasework 1.
+  intros [[[s ex] mu] a].
+  induction a.
+  2-6: split; intros [[[s' ex'] mu'] y] H; simpl in H; destruct H.
+  - split; intros [[[s' ex'] mu'] y] H; simpl in H.
+    case_match.
+    rewrite (eq_existT_curried e H). exact IHa.
+    destruct H.
+  - split; intros [[[s' ex'] mu'] y] H; simpl in H.
+    case_match.
+    destruct H.
+    rewrite (eq_existT_curried e H). exact IHa1.
+    rewrite (eq_existT_curried e H). exact IHa2.
+    destruct H.
+  - split; intros [[[s' ex'] mu'] y] H; simpl in H.
+    case_match.
+    2: destruct H.
+    induction args.
+    destruct H.
+    destruct H.
+    2: apply IHargs, H.
+    clear IHargs.
+    case_match.
+    2: destruct H.
+    enough (@existT _ (uncurry3 OPMLClosedPattern) (s', ex', mu') y = existT (x, ex, mu) f).
+    rewrite H2.
+    (* It doesn't. And I don't know why. *)
+    (* apply pleasework. Guarded. *)
+    Search eq_rect.
+    Search (eq_rect _ _ (eq_rect _ _ _ _ _) _ _).
+    pose proof (eq_existT_curried e0 H).
+Abort.
 
 Goal forall {Σ : OPMLSignature}, well_founded SubPatternOf.
 Proof.
+  intros.
+  unfold well_founded.
+  fix pleasework 1.
+  intros. destruct a as [[[s ex] mu] a].
+  destruct a.
+  8: {
+    split.
+    dependent induction args; intros.
+    - (*inversion H; subst.*)
+      dependent induction H.
+
+      inversion_sigma.
+      Search hyp:eq_rect.
+      Search hyp:eq_dep1.
+
+
   intros. split.
   destruct a as [[[s ex] mu] a].
   induction a; intros.
@@ -307,8 +440,8 @@ Proof.
   intros.
   Search Acc.
   (* dependent induction H. *)
-  inversion H; subst.
-  split. intros.
+  (* inversion H; subst. *)
+  (* split. intros. *)
   (* inversion H0; subst. *)
   (* destruct a as [[[s ex] mu] a]. *)
   (* dependent induction a. *)
@@ -329,16 +462,18 @@ Admitted.
 (*   measure_OCP (ocp_fevar x) => 0 ; *)
 (*   measure_OCP (ocp_fsvar X) => 0 ; *)
 (*   measure_OCP (ocp_imp φ1 φ2) => measure_OCP φ1 + measure_OCP φ2 ; *)
-(*   (1* measure_OCP (ocp_app σ args) => _ (*dephlist_foldr (λ _ a c, measure_OCP a + c) 0 args*) ; *1) *)
-(*   measure_OCP (ocp_app σ dhnil) => 0 ; *)
-(*   measure_OCP (ocp_app σ (dhcons x xs)) => measure_OCP x + measure_OCP (ocp_app σ xs) ; *)
+(*   measure_OCP (ocp_app σ args) => _ (*dephlist_foldr (λ _ a c, measure_OCP a + c) 0 args*) ; *)
+(*   (1* measure_OCP (ocp_app σ dhnil) => 0 ; *1) *)
+(*   (1* measure_OCP (ocp_app σ (dhcons x xs)) => measure_OCP x + measure_OCP (ocp_app σ xs) ; *1) *)
 (*   measure_OCP (ocp_ex φ) => measure_OCP φ ; *)
 (*   measure_OCP (ocp_mu φ) => measure_OCP φ ; *)
 (*   . *)
 (* Proof. *)
-(*   refine (dephlist_foldr _ 0 args). *)
-(*   intros. apply plus. eapply measure_OCP. exact X. exact H. *)
+(*   exact (dephlist_foldr (λ _ c a, measure_OCP Σ _ xs ys c + a) 0 args). *)
 (* Defined. *)
+(*   (1* refine (dephlist_foldr _ 0 args). *1) *)
+(*   (1* intros. apply plus. eapply measure_OCP. exact X. exact H. *1) *)
+(* (1* Defined. *1) *)
 
 Section asd.
 Context {Σ : OPMLSignature}.
