matching-logic/src/OPML/RT.v
@@ -1,0 +1,84 @@
+From stdpp Require Import base tactics.
+From Coq Require Import Lists.List.
+Import ListNotations.
+
+Inductive hlist {A : Type} (F : A -> Type) : list A -> Type :=
+  | hnil : hlist F []
+  | hcons {x} {xs} : F x -> hlist F xs -> hlist F (x :: xs)
+.
+
+Arguments hlist {_} _ & _.
+Arguments hnil {_} {_}.
+Arguments hcons {_} {_} {_} {_} & _ _.
+
+Declare Scope hlist_scope.
+Delimit Scope hlist_scope with hlist.
+Bind Scope hlist_scope with hlist.
+
+Infix "::" := hcons (at level 60, right associativity) : hlist_scope.
+Notation "[ ]" := hnil (format "[ ]") : hlist_scope.
+Notation "[ x ]" := (hcons x hnil) : hlist_scope.
+Notation "[ x ; y ; .. ; z ]" := (hcons x (hcons y .. (hcons z hnil) ..)) (format "[ '[' x ; '/' y ; '/' .. ; '/' z ']' ]") : hlist_scope.
+
+Check [1; 2; true; 3; false]%hlist : hlist (bool_rect _ nat bool) [true; true; false; true; false].
+
+Class Sort : Type := {
+  carrier : Type;
+  sort_ed : EqDecision carrier;
+  }.
+
+Instance asd : Sort := {| carrier := bool; sort_ed := _ |}.
+
+Inductive RT {A : Sort} (B : carrier) : Type :=
+  | Leaf : RT B
+  | Node {xs} : hlist RT xs -> RT B
+.
+
+Arguments Leaf {_} {_}.
+Arguments Node {_} {_} {_} & _.
+
+Check Node [Leaf; Node [Leaf; Leaf]; Leaf] : @RT asd true.
+
+Fixpoint depth {A} (x : RT A) : nat :=
+  match x with
+  | Leaf => 1
+  | Node l => hlist_rect _ _ _ 0 (fun _ _ y _ IHys => Nat.max IHys (depth y)) _ l
+  end.
+
+Arguments depth {_} !_.
+
+Definition hlistIn {A} {ED : EqDecision A} {F : A -> Type} {x : A} {xs : list A} (y : F x) (ys : hlist F xs) : Prop :=
+  match ys with
+  | hnil => False
+  | @hcons _ _ x' _ y' ys' => match (decide (x = x')) with
+                              | left e => (eq_rect _ _ y _ e = y')
+                              | _ => False
+                              end
+  end.
+
+Arguments hlistIn {_} {_} {_} {_} {_} & _ !_.
+
+Definition SubTree {A : Sort} {B : carrier} (x y : RT B) : Prop :=
+  match y with
+  | Leaf => False
+  | Node l => @hlistIn _ (sort_ed) _ _ _ x l
+  end.
+
+Arguments SubTree {_} {_} _ !_.
+
+Goal forall {A : Sort} {B : carrier}, well_founded (@SubTree A B).
+Proof.
+  intros.
+  unfold well_founded.
+  fix thisworks 1.
+  intros [].
+  split. intros. destruct H.
+  split. intros. simpl in H. destruct h.
+  destruct H.
+  simpl in H.
+  case_match.
+  2: destruct H.
+  apply rew_swap in H. rewrite H.
+  apply thisworks.
+Qed.
+
